```agda

{-# OPTIONS --rewriting --without-K --allow-unsolved-metas #-}

open import new-prelude

open import Lecture4-notes
open import Lecture5-notes
open import Solutions5-dan using (PathOver-path≡)

module Lecture6-live where

{- remember the definition of S1 from Lectures 4 and 5

  S1 : Type
  base : S1
  loop : base ≡ base

  For {l : Level} {X : Type l} (x : X) (p : x ≡ x)
    S1-rec : S1 → X
    S1-rec-base : S1-rec x p base ≡ x
    S1-rec-loop : ap (S1-rec x p) loop ≡ p

  For {l : Level} (X : S1 → Type l)
      (x : X base)
      (p : x ≡ x [ X ↓ loop )]
    S1-elim : (x : S1) → X x
    S1-elim-base : S1-elim X x p base ≡ x
    S1-elim-loop : apd (S1-elim X x p) loop ≡ p

-}

Ω¹S1 : Type
Ω¹S1 = {!!}

Ω²S1 : Type
Ω²S1 = {!!}

{-
Correspondence

-2
-1
 0
 1
 2
-}

module AssumeInts 
    (ℤ : Type)
    (0ℤ : {!!})
    (succℤ : {!!})
    (ℤ-rec : {!!})
    (ℤ-rec-0ℤ : {X : Type}
                (b : X)
                (s : X ≃ X)
                → {!!})
    (ℤ-rec-succℤ : {X : Type}
                   (b : X)
                   (s : X ≃ X)
                   → {!!})
    (ℤ-rec-unique : {X : Type}
                    (f : ℤ → X)
                    (z : X)
                    (s : X ≃ X)
                  → {!!}
                  → {!!}
                 → (x : ℤ) → f x ≡ {!!})
    where



  loop^ : ℤ → base ≡ base
  loop^ = {!!}

  encode-firsttry : base ≡ base → ℤ
  encode-firsttry = {!!}

  Cover : S1 → Type
  Cover = {!!}

  encode : (x : S1) → base ≡ x → Cover x
  encode = {!!}

  encode-loop^ : (x : ℤ) → encode base (loop^ x) ≡ x
  encode-loop^ = {!!}

  endo-ℤ-is-id : (f : ℤ → ℤ)
               → {!!}
               → {!!}
               → f ∼ id
  endo-ℤ-is-id = {!!}

  loop^-encode : (p : base ≡ base) → loop^ (encode base p) ≡ p
  loop^-encode = {!!}

  PathOver-→ : {X : Type}
               {A : X → Type}
               {B : X → Type}
               {x x' : X} {p : x ≡ x'}
               {f1 : A x → B x}
               {f2 : A x' → B x'}
             → {!!}
             → f1 ≡ f2 [ (\ z → A z → B z) ↓ p ]
  PathOver-→ {A = A} {B} {p = p} {f2 = f2} h = {!!}

  PathOver-path-to : ∀ {A : Type} 
                       {a0 a a' : A} {p : a ≡ a'}
                       {q : a0 ≡ a}
                       {r : a0 ≡ a'}
                      → {!!}
                      → q ≡ r [ (\ x → a0 ≡ x) ↓ p ]
  PathOver-path-to = {!!}

  decode : (x : S1) → Cover x → base ≡ x
  decode = {!!}

  encode-decode : (x : S1) (p : base ≡ x) → decode x (encode x p) ≡ p
  encode-decode = {!!}

  theorem : (base ≡ base) ≃ ℤ
  theorem = improve (Isomorphism (encode base) (Inverse loop^ loop^-encode encode-loop^))

  -- prove PathOver-→
  -- implement ℤ
  -- extend encode-loop^

```

